Closer to getting substitution working with typed terms

ling.v
@@ -1,26 +1,90 @@
 Require Import Bool Arith List.
 Require Import Coq.Program.Equality.
+Require Import Program.
 Load hlist.
 Load syntax.
 Set Implicit Arguments.
 Set Asymmetric Patterns.
 
 Example inc : exp nil (TList TNat) :=
-  emap (eplus (evar HFirst) (econst 3)) (econs (econst 4) enil).
+  emap (eplus (evar zvar) (econst 3)) (econs (econst 4) enil).
 
 Example let_ex : exp nil TNat :=
-  elet (econst 42) (eplus (evar HFirst) (econst 10)).
+  elet (econst 42) (eplus (evar zvar) (econst 10)).
 
 Example app_prog : exp nil (TList TNat) := eappend (econs (econst 0) enil) (econs (econst 1) enil).
 
 Example nested_map : exp nil (TList TNat) :=
-  emap (eplus (econst 3) (evar HFirst))
-  (emap (eplus (evar HFirst) (econst 10)) [| econst 1 ; econst 2 ; econst 3 |]).
+  emap (eplus (econst 3) (evar zvar))
+  (emap (eplus (evar zvar) (econst 10)) [| econst 1 ; econst 2 ; econst 3 |]).
 
 Example flat_map : exp nil (TList TNat) :=
-  emap (eplus (econst 3) (eplus (evar HFirst) (econst 10)))
+  emap (eplus (econst 3) (eplus (evar zvar) (econst 10)))
        [| econst 1 ; econst 2 ; econst 3 |].
 
+Definition Sub G G' := forall t, var G t -> exp G' t. 
+
+Definition idSub {G} : Sub G G := @evar G.
+
+Program Definition consSub {G G' t} (e:exp G' t) (s:Sub G G') : Sub (t::G) G' :=
+  fun t' (v: var (t::G) t') =>
+    match v with
+    | zvar _ _ => e
+    | svar _ _ _ v' => s _ v'
+    end.
+    
+Notation "{| e ; .. ; f |}" := (consSub e .. (consSub f idSub) ..).
+
+Definition Ren G G' := forall t, var G t -> var G' t.
+
+Program Definition renameLift {G G' t}
+        (r : Ren G G') : Ren (t :: G) (t :: G') :=
+  fun t' v =>
+    match v with
+    | zvar _ _ => zvar
+    | svar _ _ _ v' => svar (r _ v')
+    end.
+
+Fixpoint renameExp G G' t (r : Ren G G') (e : exp G t) :=
+  match e with
+  | evar _ x => evar (r _ x)
+  | etrue => etrue
+  | efalse => efalse
+  | econst n => econst n
+  | eplus e1 e2 => eplus (renameExp r e1) (renameExp r e2)
+  | enil _ => enil
+  | econs _ e1 e2 => econs (renameExp r e1) (renameExp r e2)
+  | elet _ _ e1 e2 => elet (renameExp r e1) (renameExp (renameLift r) e2)
+  | eappend _ e1 e2 => eappend (renameExp r e1) (renameExp r e2)
+  | emap _ _ e1 e2 => emap (renameExp (renameLift r) e1) (renameExp r e2)
+  | efilter _ e1 e2 => efilter (renameExp (renameLift r) e1) (renameExp r e2)
+  end.
+
+Definition shiftExp G t t' : exp G t -> exp (t' :: G) t :=
+  renameExp (fun _ v => svar v).
+
+Program Definition
+        subShift {G G'} t (s : Sub G G') : Sub (t :: G) (t :: G') :=
+  fun t' v =>
+    match v with
+    | zvar _ _ => evar zvar
+    | svar _ _ _ v' => shiftExp t (s _ v')
+    end.
+
+Fixpoint subExp G G' t (s : Sub G G') (e : exp G t) :=
+  match e with
+  | evar _ x => s _ x
+  | etrue => etrue
+  | efalse => efalse
+  | econst n => econst n
+  | eplus e1 e2 => eplus (subExp s e1) (subExp s e2)
+  | enil _ => enil
+  | econs _ e1 e2 => econs (subExp s e1) (subExp s e2)
+  | elet _ _ e1 e2 => elet (subExp s e1) (subExp (subShift s) e2)
+  | eappend _ e1 e2 => eappend (subExp s e1) (subExp s e2)
+  | emap _ _ e1 e2 => emap (subExp (subShift s) e1) (subExp s e2)
+  | efilter _ e1 e2 => efilter (subExp (subShift s) e1) (subExp s e2)
+  end.
 
 Fixpoint tyDenote (t : ty) : Type :=
   match t with
@@ -38,82 +102,43 @@ Fixpoint valDenote t (v : val t) : tyDenote t :=
   | vcons _ v1 v2 => (valDenote v1) :: (valDenote v2)
   end.
 
+Fixpoint envDenote G : Type :=
+  match G with
+  | nil => unit
+  | t :: G => prodT (tyDenote t) (envDenote G)
+  end.
+
+Fixpoint getVar G t (v : var G t) : envDenote G -> tyDenote t :=
+  match v with
+  | zvar _ _ => fun se => fst se
+  | svar _ _ _ v => fun se => getVar v (snd se)
+  end.
+
 (* An interpreter *)
-Fixpoint expDenote G t (e : exp G t) : hlist tyDenote G -> tyDenote t :=
+Fixpoint expDenote G t (e : exp G t) : envDenote G -> tyDenote t :=
   match e with
-  | evar _ _ x => fun s => hget s x
-  | econst _ n => fun _ => n
-  | etrue _ => fun _ => true
-  | efalse _ => fun _ => false
-  | eplus _ e1 e2 => fun s => (expDenote e1 s) + (expDenote e2 s)
-  | enil _ _ => fun _ => nil
-  | econs _ _ e1 e2 => fun s => (expDenote e1 s) :: (expDenote e2 s)
-  | elet _ _ _ e el =>
-    fun s => expDenote el (HCons (expDenote e s) s)
-  | eappend _ _ e1 e2 => fun s => app (expDenote e1 s) (expDenote e2 s)
-  | emap _ _ _ ef e =>
-    fun s => let f := fun x => expDenote ef (HCons x s)
+  | evar _ x => getVar x
+  | econst n => fun _ => n
+  | etrue => fun _ => true
+  | efalse => fun _ => false
+  | eplus e1 e2 => fun s => (expDenote e1 s) + (expDenote e2 s)
+  | enil _ => fun _ => nil
+  | econs _ e1 e2 => fun s => (expDenote e1 s) :: (expDenote e2 s)
+  | elet _ _ e el =>
+    fun s => expDenote el ((expDenote e s), s)
+  | eappend _ e1 e2 => fun s => app (expDenote e1 s) (expDenote e2 s)
+  | emap _ _ ef e =>
+    fun s => let f := fun x => expDenote ef (x, s)
              in map f (expDenote e s)
+  | efilter _ ef e =>
+    fun s => let f := fun x => expDenote ef (x, s)
+             in filter f (expDenote e s)
   end.
 
-Eval compute in (expDenote app_prog) HNil.
-Eval compute in (expDenote let_ex) HNil.
-Eval compute in (expDenote inc) HNil.
+Eval compute in (expDenote app_prog) ().
+Eval compute in (expDenote let_ex) ().
+Eval compute in (expDenote inc) ().
 
-Fixpoint insertAt (t : ty) (G : list ty) (n : nat) {struct n}
-  : list ty :=
-  match n with
-  | O => t :: G
-  | S n' => match G with
-            | nil => t :: G
-            | t' :: G' => t' :: insertAt t G' n'
-            end
-  end.
-
-Fixpoint liftVar t G (x : member t G) t' n
-  : member t (insertAt t' G n) :=
-  match x with
-  | HFirst G' => match n return member t (insertAt t' (t :: G') n) with
-                 | O => HNext HFirst
-                 | _ => HFirst
-                 end
-  | HNext t'' G' x' => match n return member t (insertAt t' (t'' :: G') n) with
-                       | O => HNext (HNext x')
-                       | S n' => HNext (liftVar x' t' n')
-                       end
-  end.
-
-Fixpoint lift' G t' n t (e : exp G t) : exp (insertAt t' G n) t :=
-  match e with
-  | evar _ _ x => evar (liftVar x t' n)
-  | etrue _ => etrue
-  | efalse _ => efalse
-  | econst _ n => econst n
-  | eplus _ e1 e2 => eplus (lift' t' n e1) (lift' t' n e2)
-  | enil _ _ => enil
-  | econs _ _ e1 e2 => econs (lift' t' n e1) (lift' t' n e2)
-  | elet _ _ _ e el => elet (lift' t' n e) (lift' t' (S n) el)
-  | eappend _ _ e1 e2 => eappend (lift' t' n e1) (lift' t' n e2)
-  | emap _ _ _ ef e => emap (lift' t' (S n) ef) (lift' t' n e)
-  end.
-
-Definition lift G t' t (e : exp G t) : exp (t' :: G) t :=
-  lift' t' O e.
-
-Check @HFirst.
-
-
-Eval simpl in lift (TBool) (eplus (econst 10) (evar HFirst)).
-
-(* Substitute ef' for all occurences of x in ef *)
-
-Fixpoint subst_first G t t1 t2
-         (ef' : exp (t1 :: G) t2)
-         (ef : exp (t2 :: G) t)
-  : exp (t1 :: G) t.
-  Admitted.
-  
-Check subst_first.
 
 Lemma append_assoc : forall G t (e1 e2 e3: exp G (TList t)) s,
     expDenote (eappend (eappend e1 e2) e3) s =
@@ -134,12 +159,22 @@ Qed.
  * replace all occurences of x in f by result of g
  *)
 
-Definition fuse_map G t (e : exp G t): exp G t :=
-  match e with
-  | emap _ _ _ ef eb => emap ef eb
-  | _ => e
-  end.
-      
+Print nested_map.
+
+Eval simpl in subExp {| econst 10; econst 20 |} (eplus (evar zvar) (evar (svar zvar))).
+
+Example nested_map' : exp nil (TList TNat) :=
+  emap (eplus (econst 3) (evar zvar))
+  (emap (eplus (evar zvar) (econst 10)) [| econst 1 ; econst 2 ; econst 3 |]).
+
+Example f1 : exp (TNat :: nil) (TList TNat) := (econs (evar zvar) enil).
+Example f2 : exp (TNat :: nil) TNat := (eplus (evar zvar) (econst 10)).
+
+Check (subExp {| f2 |} (shiftExp _ f1)).
+
+Eval simpl in expDenote (emap f1 (emap f2 [| econst 10; econst 20; econst 30 |])).
+Eval simpl in expDenote (emap (subExp {| f2 |} (shiftExp _ f1)) [| econst 10; econst 20; econst 30 |]).
+
 (* Inductive judgment for append *)
 Inductive CApp : forall t,
     val (TList t) -> val (TList t) -> val (TList t) -> Prop :=
