syntax.v
@@ -3,18 +3,28 @@ Inductive ty : Type :=
 | TNat : ty
 | TList : ty -> ty.
 
+Definition env := list ty.
+
+Inductive var : env -> ty -> Type :=
+| zvar : forall G t, var (t :: G) t
+| svar : forall G t t', var G t -> var (t' :: G) t.
+
+Arguments zvar [G t].
+Arguments svar [G t t'].
+
 (* Intrinsically typed expression syntax *)
-Inductive exp : list ty -> ty -> Type :=
-| evar : forall G t, member t G -> exp G t
-| etrue : forall G, exp G TBool
-| efalse : forall G, exp G TBool
-| econst : forall G, nat -> exp G TNat
-| eplus : forall G, exp G TNat -> exp G TNat -> exp G TNat
-| enil : forall G t, exp G (TList t)
-| econs : forall G t, exp G t -> exp G (TList t) -> exp G (TList t)
-| elet : forall G t1 t2, exp G t1 -> exp (t1 :: G) t2 -> exp G t2
-| eappend : forall G t, exp G (TList t) -> exp G (TList t) -> exp G (TList t)
-| emap : forall G t1 t2, exp (t1 :: G) t2 -> exp G (TList t1) -> exp G (TList t2).
+Inductive exp G : ty -> Type :=
+| evar : forall t, var G t -> exp G t
+| etrue : exp G TBool
+| efalse : exp G TBool
+| econst : nat -> exp G TNat
+| eplus : exp G TNat -> exp G TNat -> exp G TNat
+| enil : forall t, exp G (TList t)
+| econs : forall t, exp G t -> exp G (TList t) -> exp G (TList t)
+| elet : forall t1 t2, exp G t1 -> exp (t1 :: G) t2 -> exp G t2
+| eappend : forall t, exp G (TList t) -> exp G (TList t) -> exp G (TList t)
+| emap : forall t1 t2, exp (t1 :: G) t2 -> exp G (TList t1) -> exp G (TList t2)
+| efilter : forall t1, exp (t1 :: G) TBool -> exp G (TList t1) -> exp G (TList t1).
 
 Arguments econst [G].
 Arguments etrue [G].
