simple/proofs.v
@@ -1,0 +1,61 @@
+Set Implicit Arguments.
+Set Asymmetric Patterns.
+
+Inductive bool : Set := true : bool | false : bool.
+
+Definition and (b1 b2 : bool) : bool :=
+  match b1 with
+  | false => false
+  | true => b2
+  end.
+
+Inductive list (T : Set) : Set :=
+| nil : list T
+| cons : T -> list T -> list T.
+
+Arguments nil [T].
+Arguments cons [T].
+
+Fixpoint map (T T' : Set) (f : T -> T') (ls : list T) : list T' :=
+  match ls with
+  | nil => nil
+  | cons x ls' => cons (f x) (map f ls')
+  end.
+
+Fixpoint filter (T : Set) (p : T -> bool) (ls : list T) : list T :=
+  match ls with
+  | nil => nil
+  | cons x ls' => if p x then cons x (filter p ls') else filter p ls'
+  end.
+
+Theorem map_fusion : forall (T T' T'' : Set) (f : T' -> T'')
+                            (g : T -> T') (ls : list T),
+    map f (map g ls) = map (fun x => f (g x)) ls.
+  induction ls. reflexivity.
+  simpl. rewrite <- IHls. reflexivity.
+Qed.
+
+Lemma and_true_r : forall b : bool,
+    and b true = b.
+  intros.
+  destruct b; reflexivity.
+Qed.
+
+Lemma and_false_r : forall b : bool,
+    and b false = false.
+  intros.
+  destruct b; reflexivity.
+Qed.
+
+Lemma filter_fusion : forall (T : Set) (p q : T -> bool)
+                             (ls : list T),
+    filter p (filter q ls) = filter (fun x => and (p x) (q x)) ls.
+  induction ls. reflexivity. simpl.
+  destruct (q t); simpl.
+  rewrite IHls. rewrite (and_true_r (p t)).
+  reflexivity.
+  rewrite (and_false_r (p t)). rewrite IHls.
+  reflexivity.
+Qed.
+
+
