untyped/debruijn.v
@@ -1,0 +1,225 @@
+Require Import Coq.Arith.Arith.
+Require Import Coq.Bool.Bool.
+Require Import Coq.Strings.String.
+Require Import Coq.Lists.List
+Require Import Coq.Logic.FunctionalExtensionality.
+
+Inductive ty : Type :=
+| TBool : ty
+| TNat : ty
+| TList : ty -> ty.
+
+Inductive exp : Type :=
+| evar : nat -> exp
+| etrue : exp
+| efalse : exp
+| econst : nat -> exp
+| eplus : exp -> exp -> exp
+| enil : exp
+| econs : exp -> exp -> exp
+| eappend : exp -> exp -> exp
+| emap : exp -> exp -> exp.
+
+Inductive val : Type :=
+| vtrue : val
+| vfalse : val
+| vconst : nat -> val
+| vnil : val
+| vcons : val -> val -> val.
+
+Definition context := list ty.
+
+Inductive has_type : context -> exp -> ty -> Prop :=
+| tvar : forall G x T,
+    G x = Some T -> has_type G (evar x) T
+| ttrue : forall G, has_type G etrue TBool
+| tfalse : forall G, has_type G efalse TBool
+| tconst : forall G n, has_type G (econst n) TNat
+| tplus : forall G e1 e2, has_type G e1 TNat ->
+                          has_type G e2 TNat ->
+                          has_type G (eplus e1 e2) TNat
+| tnil : forall G t, has_type G enil (TList t)
+| tcons : forall G e e' t,
+    has_type G e t -> has_type G e' (TList t) ->
+    has_type G (econs e e') (TList t)
+| tappend : forall G e e' t,
+    has_type G e (TList t) -> has_type G e' (TList t) ->
+    has_type G (eappend e e') (TList t)
+| tmap : forall G x e el t t',
+    has_type (update G x t) e t' -> has_type G el (TList t) ->
+    has_type G (emap x e el) (TList t').
+
+Inductive val_has_type : val -> ty -> Prop :=
+| vttrue : val_has_type vtrue TBool
+| vtfalse : val_has_type vfalse TBool
+| vtconst : forall n, val_has_type (vconst n) TNat
+| vtnil : forall t, val_has_type vnil (TList t)
+| vtcons : forall v v' t,
+    val_has_type v t -> val_has_type v' (TList t) ->
+    val_has_type (vcons v v') (TList t).
+
+Definition env := partial_map val.
+
+Inductive eval : env -> exp -> val -> Prop :=
+| ev_var : forall G x v,
+    G x = Some v -> eval G (evar x) v
+| ev_true : forall G, eval G etrue vtrue
+| ev_false : forall G, eval G efalse vfalse
+| ev_const : forall G n, eval G (econst n) (vconst n)
+| ev_plus : forall G e1 e2 n1 n2,
+    eval G e1 (vconst n1) -> eval G e2 (vconst n2) ->
+    eval G (eplus e1 e2) (vconst (n1 + n2))
+| ev_nil : forall G, eval G enil vnil
+| ev_cons : forall G e1 e2 v1 v2, eval G e1 v1 -> eval G e2 v2 ->
+                                  eval G (econs e1 e2) (vcons v1 v2).
+
+Definition x := (Id "x").
+Definition y := (Id "y").
+Definition z := (Id "z").
+Hint Unfold x.
+Hint Unfold y.
+Hint Unfold z.
+
+Hint Constructors has_type.
+
+Example typing :
+  has_type empty (eplus (econst 10) (econst 20)) TNat.
+Proof.
+  auto.
+Qed.
+
+Hint Immediate tplus.
+
+Example typing1 :
+  has_type empty (emap x (eplus (evar x) (econst 10)) (econs (econst 10) (econs (econst 20) enil))) (TList TNat).
+Proof.
+  eapply tmap.
+  apply tplus.
+  apply tvar.
+  rewrite update_eq.
+  reflexivity.
+  apply tconst.
+  auto.
+Qed.
+
+(* substitute x with s in t *)
+Fixpoint subst (x:id) (s:exp) (e:exp) : exp :=
+  match e with
+  | evar x' => if beq_id x x' then s else e
+  | etrue => etrue
+  | efalse => efalse
+  | econst n => econst n
+  | eplus e1 e2 => eplus (subst x s e1) (subst x s e2)
+  | enil => enil
+  | econs e1 e2 => econs (subst x s e1) (subst x s e2)
+  | eappend e1 e2 => eappend (subst x s e1) (subst x s e2)
+  | emap x' e1 e2 => emap x' (if beq_id x x' then e1 else (subst x s e1))
+                          (subst x s e2)
+  end.
+
+Inductive appears_free_in : id -> exp -> Prop :=
+| afi_var : forall x, appears_free_in x (evar x)
+| afi_plus1 : forall x e1 e2, appears_free_in x e1 -> appears_free_in x (eplus e1 e2)
+| afi_plus2 : forall x e1 e2, appears_free_in x e2 -> appears_free_in x (eplus e1 e2)
+| afi_cons1 : forall x e1 e2, appears_free_in x e1 -> appears_free_in x (econs e1 e2)
+| afi_cons2 : forall x e1 e2, appears_free_in x e2 -> appears_free_in x (econs e1 e2)
+| afi_app1 : forall x e1 e2, appears_free_in x e1 -> appears_free_in x (eappend e1 e2)
+| afi_app2 : forall x e1 e2, appears_free_in x e2 -> appears_free_in x (eappend e1 e2)
+| afi_map1 : forall x y e1 e2, x <> y -> appears_free_in x e1 -> appears_free_in x (emap y e1 e2)
+| afi_map2 : forall x e1 e2, appears_free_in x e2 -> appears_free_in x (emap x e1 e2).
+                                                                      
+
+Lemma free_in_context : forall x e T G,
+    appears_free_in x e ->
+    has_type G e T ->
+    exists T', G x = Some T'.
+  intros. generalize dependent G.
+  generalize dependent T.
+  induction H; intros;
+    try (inversion H0; eauto);
+    inversion H1;
+    subst;
+    try (match goal with
+         | [ H : has_type _ _ _ |- _ ] => apply IHappears_free_in in H;
+                                          rewrite update_neq in H
+                                                                  
+         end);
+    auto.
+Qed.
+
+Lemma empty_is_empty : forall A (x : id), (empty : partial_map A) x = None.
+  Proof.
+    intros.
+    unfold empty.
+    unfold t_empty.
+    reflexivity.
+Qed.
+
+Lemma ev_preserves_type : forall e v T,
+    has_type empty e T -> eval empty e v -> val_has_type v T.
+  intros.
+  generalize dependent H0.
+  induction H; intros; inversion H0; subst.
+  rewrite empty_is_empty in H3.
+  inversion H3.
+  constructor.
+  constructor.
+  constructor.
+  
+
+
+
+
+
+
+
+
+  
+
+
+Lemma subst_preserves_type : forall G x T' e e' T,
+    has_type (update G x T') e T ->
+    has_type empty e' T' ->
+    has_type G (subst x e' e) T.
+Proof.
+  intros G x T' e e' T.
+  generalize dependent G. generalize dependent T.
+  induction e; intros T G H; inversion H;
+    subst; simpl.
+  destruct (beq_id x i).
+
+
+  
+Definition map_fusion (e : exp) : exp :=
+  match e with
+  | emap x f list =>
+    match list with
+    | emap y g list' => emap y (subst x g f) list'
+    | _ => e
+    end
+  | _ => e
+  end.
+
+Example nested_map := emap x (eplus (evar x) (econst 10)) (emap x (eplus (econst 5) (evar x)) (econs (econst 10) (econs (econst 20) enil))).
+
+Eval simpl in (map_fusion nested_map).
+
+Lemma map_fusion_type_preservation : forall e t, has_type empty e t -> has_type empty (map_fusion e) t.
+  intros.
+  induction e;
+    destruct t;
+    try (unfold map_fusion; assumption).
+  inversion H.
+  inversion H.
+  
+
+
+
+  
+
+  
+
+  
+
+  
+
